add vars

Spacetalk/SimpleArith.lean
@@ -1,20 +1,34 @@
 import Mathlib.Data.Stream.Defs
+import Mathlib.Data.Vector3
+import Mathlib.Tactic.SimpRw
 import Aesop
+
+def Vector.nil_append : ∀ vNil : Vector α 0, ∀ v : Vector α n, vNil.append v = v.cast (Nat.zero_add n).symm := by
+  intro vNil v
+  simp only [Vector.append, mk_eq, toArray_cast, Array.append_left_eq_self, toArray_eq_empty_iff]
 
 def Vector.split (v : Vector α (n + m)) : Vector α n × Vector α m :=
   have h_min_eq : min n (n + m) = n := Nat.min_add_right
   have h_minus_eq : n + m - n = m := by omega
   (h_min_eq ▸ (v.take n), h_minus_eq ▸ (v.drop n))
 
-inductive Exp
-  | val : Nat → Exp
-  | plus : Exp → Exp → Exp
+inductive Exp : Nat → Type
+  | val : Nat → Exp 0
+  | var : Exp 1
+  | plus : Exp inp1 → Exp inp2 → Exp (inp1 + inp2)
 
-def Exp.eval : Exp → Nat
-| .val v => v
-| .plus e1 e2 => e1.eval + e2.eval
+def Exp.eval : Exp inp → Vector Nat inp → Nat
+| (.val v), _ => v
+| .var, inp => inp[0]
+| (.plus e1 e2), inp =>
+  let (inp1, inp2) := inp.split
+  (e1.eval inp1) + (e2.eval inp2)
 
-def Exp.denote (e : Exp) : Stream' Nat := .const (e.eval)
+def Vector.packStreams (ss : Vector (Stream' α) len) : Stream' (Vector α len) :=
+  λ n => ss.map (·.get n)
+
+def Exp.denote (e : Exp inp) (inpVals : Vector (Stream' Nat) inp) : Stream' Nat :=
+  λ n => (e.eval) (inpVals.packStreams n)
 
 -- single output only
 inductive Node (α : Type) : Nat → Type
@@ -39,35 +53,63 @@ def Graph.denote : Graph (Stream' Nat) nInp → (Vector (Stream' Nat) nInp) → 
   let (μNodeInp, fInp) := vInp.split
   (f (n.denote μNodeInp)).denote fInp
 
-def Exp.compileC (cont : α → Graph α n) : Exp → Graph α n
-| .val v => .μClosed (.val v) #v[] cont
-| .plus e1 e2 =>
-  e1.compileC λ e1Out =>
-  e2.compileC λ e2Out =>
-  .μClosed .plus #v[e1Out, e2Out] cont
+def Exp.compileC (cont : α → Graph α nCont) : Exp nExp → Graph α (nExp + nCont)
+| .val v => (Nat.zero_add nCont).symm ▸ .μClosed (.val v) #v[] cont
+| .var => .μOpen .id cont
+| @Exp.plus inp1 inp2 e1 e2 =>
+  have : inp1 + (inp2 + nCont) = inp1 + inp2 + nCont := by omega
+  this ▸
+    (e1.compileC λ e1Out =>
+     e2.compileC λ e2Out =>
+     .μClosed .plus #v[e1Out, e2Out] cont)
 
-def Exp.compile (e : Exp) : Graph α 0 :=
+theorem graph_subst {n m : Nat} {h : n = m} {g1 : Graph (Stream' Nat) n}
+  : (h ▸ g1).denote = h ▸ g1.denote := by
+  subst h
+  simp_all only
+
+def Exp.compile (e : Exp n) : Graph α n :=
   e.compileC λ out => .nodeClosed .id #v[out]
 
 theorem compileC_correct
-  : ∀ e : Exp, ∀ f : _ → Graph _ n,
-    (f e.denote).denote = (e.compileC f).denote := by
-  intro e f
+  : ∀ e : Exp nExp, ∀ f : Stream' Nat → Graph _ nCont,
+    ∀ vInpExp : Vector (Stream' Nat) nExp, ∀ vInpCont : Vector (Stream' Nat) nCont,
+    (f (e.denote vInpExp)).denote vInpCont = (e.compileC f).denote (vInpExp.append vInpCont) := by
+  intro e f vInpExp vInpCont
   induction e generalizing f with
   | val v =>
+    funext i
     simp only [Exp.denote, Stream'.const, Exp.eval, Exp.compileC, Graph.denote, Node.denote,
       Vector.getElem_mk, List.getElem_toArray, List.getElem_cons_zero]
+    rw [Eq.rec_eq_cast]
+    -- induction nCont with
+    -- | zero =>
+    --   cases congr_arg (Graph (Stream' ℕ)) Exp.compileC.proof_6
+    --   simp [Graph.denote, Node.denote]
+    --   unfold Exp.denote
+    --   simp [Exp.eval]
+    --   unfold Stream'.const
+    --   cases vInpCont
+    --   cases vInpExp
+    --   simp [Vector.append]
+    --   rename_i heq
+    --   simp_rw [Array.size_eq_zero_iff.mp heq]
+    --   simp_rw [Array.empty_append]
+    -- | succ n ih =>
+    -- cases (congr_arg (Graph (Stream' ℕ)) Exp.compileC.proof_6)
+    cases h : Graph.μClosed (Node.val v) #v[] f
+    · contradiction
+    · rename_i node inpVec cont
+      rw [Vector.nil_append vInpExp vInpCont]
+      -- cases Eq.symm (Nat.zero_add nCont)
+      -- cases congr_arg (Graph (Stream' ℕ)) Exp.compileC.proof_6
+      -- have : 0 + nCont = nCont := by aesop
+      -- rw [this]
+      -- cases @cast (Graph (Stream' ℕ) nCont) (Graph (Stream' ℕ) (0 + nCont)) (congr_arg (Graph (Stream' ℕ)) Exp.compileC.proof_6) (Graph.μClosed node inpVec cont)
+      sorry
+    · contradiction
+
+  | var => sorry
   | plus e1 e2 ih1 ih2 =>
     simp only [Exp.denote, Exp.eval, Exp.compile, Stream'.const, Exp.compileC]
-    rw [←ih1]
-    rw [←ih2]
-    simp only [Graph.denote]
-    rfl
-
-theorem compile_correct : ∀ e : Exp, e.denote = e.compile.denote #v[] := by
-  intro e
-  simp only [Exp.compile]
-  have := compileC_correct e (λ out => .nodeClosed .id #v[out])
-  rw [←this]
-  simp only [Graph.denote, Node.denote, Vector.getElem_mk, List.getElem_toArray,
-    List.getElem_cons_zero]
+    sorry
